finish lemma's in interm equivalence proof

theories/equivalence/proof.v
@@ -1,22 +1,63 @@
 From stdpp Require Import base list.
 From Autosubst Require Export Autosubst.
 Require Export Utf8_core.
-From fae_gtlc_mu.equivalence Require Import types consistency_standard consistency_intermediate wf_order upper_bound.
+From fae_gtlc_mu.equivalence Require Import types consistency_standard consistency_intermediate upper_bound.
 Require Import Relation_Operators.
 Require Import Transitive_Closure.
 From Coq.Wellfounded Require Import Lexicographic_Product Union.
 From Coq.Program Require Import Wf.
 
 
-Definition smart_lookup {A} (l : list A) (x : A) : (sum { i : nat & l !! i = Some x } (x ∉ l)).
+Lemma smart_lookup (l : list (type * type)) (x : type * type) : (sum { i : nat & l !! i = Some x } (x ∉ l)).
+Proof.
+  destruct (decide (x ∈ l)).
+  - left. admit.
+    (* destruct (elem_of_list_lookup_1 l x e) as [i eq]. *)
+  - auto.
 Admitted.
 
-(** maybe better to avoid program fixpoint altogether? *)
+Definition lexord : relation (@sigT nat (fun _ => nat)) :=
+  (lexprod _ _ lt (fun _ => lt)).
+
+Lemma ord_left n n' m m' : n < n' → lexord (existT n m) (existT n' m').
+Proof.
+  intros. by apply left_lex.
+Qed.
+
+Lemma ord_right n n' m m' : n ≤ n' → m < m' → lexord (existT n m) (existT n' m').
+Proof.
+  intros.
+  destruct (decide (n < n')).
+  - by apply left_lex.
+  - assert (triv : n = n'). lia. rewrite triv. clear triv.
+    by apply right_lex.
+Qed.
+
+Fixpoint size (τ : type) : nat :=
+  match τ with
+  | TUnit => 1
+  | TArrow τ1 τ2 => size τ1 + size τ2
+  | TRec τ => S (size τ)
+  | TVar x => 1
+  | TUnknown => 1
+  end.
+
+Lemma size_gt_0 τ : 0 < size τ.
+Proof. induction τ; simpl; lia. Qed.
+
+Definition size_pair (p : type * type) : nat :=
+  match p with | pair x x0 => size x + size x0 end.
 
 Require Import JMeq.
 
+(** TODO; remove program fixpoint... *)
+
+(* Lemma struct_validity (A : list (type * type)) (pA : Forall (fun p => TClosed p.1 ∧ TClosed p.2) A) *)
+(*       τ (pτC : TClosed τ) τ' (pτ'C : TClosed τ') (pStand : cons_stand τ τ') : cons_struct_pre A τ τ'. *)
+(* Proof. *)
+
 Program Fixpoint struct_validity (A : list (type * type)) (pA : Forall (fun p => TClosed p.1 ∧ TClosed p.2) A) τ (pτC : TClosed τ) τ' (pτ'C : TClosed τ') (pStand : cons_stand τ τ')
-        {measure (existT (upper_bound A τ τ') (τ , τ')) lexord} : cons_struct_pre A τ τ' :=
+        {measure (existT (upper_bound A τ τ') (size_pair (τ , τ'))) lexord} : cons_struct_pre A τ τ' :=
   match pStand with
   | GenSymUnit => consBaseBase A
   | GenSymUnknownL τr => _
@@ -43,18 +84,18 @@ Proof.
   - by apply consStarTGround.
   - apply consGroundArrowTau; auto.
     apply (struct_validity A pA τ1 (TArrow_closed1 pτ'C) TUnknown pτC (GenSymUnknownR τ1)).
-    { admit. }
+    { simpl. apply ord_right. apply upper_bound_le_unknown_arrow_con. pose (p := size_gt_0 τ2). lia. }
     apply (struct_validity A pA TUnknown pτC τ2 (TArrow_closed2 pτ'C) (GenSymUnknownL τ2)).
-    { admit. }
+    { simpl. apply ord_right. apply upper_bound_le_unknown_arrow_cov.  pose (p := size_gt_0 τ1). lia. }
   - destruct (smart_lookup A (TRec TUnknown , TRec τ)) as [[i p] | np].
     + by apply (consGroundRecTauUseCall A τ i).
     + apply consGroundRecTauExposeCall; auto.
       apply (struct_validity ((TRec TUnknown, TRec τ) :: A)). constructor; simpl; auto. split; auto. done. done. apply (TRec_closed_unfold pτ'C).
       assert (H : TUnknown = TUnknown.[TRec TUnknown/]). by asimpl. rewrite H.
       apply GenSymUnknownL.
-      { apply t_step. apply left_lex. simpl. apply upper_bound_lt_star_rec; auto. }
+      { simpl. apply ord_left. apply upper_bound_lt_star_rec; auto. }
   - exfalso. apply (no_var_is_closed i pτ'C).
-Admitted.
+Qed.
 
 Next Obligation.
   intros; simplify_eq.
@@ -65,31 +106,35 @@ Next Obligation.
   - by apply consTGroundStar.
   - apply consTauGroundArrow; auto.
     apply (struct_validity A pA TUnknown pτ'C τ1 (TArrow_closed1 pτC) (GenSymUnknownL τ1)).
-    { admit. }
+    { simpl. apply ord_right. apply upper_bound_le_arrow_unknown_con. pose (p := size_gt_0 τ2). lia. }
     apply (struct_validity A pA τ2 (TArrow_closed2 pτC) TUnknown pτ'C (GenSymUnknownR τ2)).
-    { admit. }
+    { simpl. apply ord_right. apply upper_bound_le_arrow_unknown_cov. pose (p := size_gt_0 τ1). lia. }
   - destruct (smart_lookup A (TRec τ , TRec TUnknown)) as [[i p] | np].
     + by apply (consTauGroundRecUseCall A τ i).
     + apply consTauGroundRecExposeCall; auto.
       apply (struct_validity ((TRec τ, TRec TUnknown) :: A)). constructor; simpl; auto. split; auto. done. apply (TRec_closed_unfold pτC). done.
       assert (H : TUnknown = TUnknown.[TRec TUnknown/]). by asimpl.
       apply GenSymUnknownR.
-      { apply t_step. apply left_lex. simpl. apply upper_bound_lt_rec_star; auto. }
+      { apply ord_left. apply upper_bound_lt_rec_star; auto. }
   - exfalso. apply (no_var_is_closed i pτC).
-Admitted.
+Qed.
 
 (** TArrow *)
 
 Next Obligation.
 Proof.
   intros; simplify_eq.
-Admitted.
+  apply ord_right. apply upper_bound_le_arrow_l. simpl.
+  pose (p := size_gt_0 τ2). lia.
+Qed.
 
 
 Next Obligation.
 Proof.
   intros; simplify_eq.
-Admitted.
+  apply ord_right. apply upper_bound_le_arrow_r.
+  simpl. pose (p1 := size_gt_0 τ1). lia.
+Qed.
 
 (** TRec *)
 
@@ -103,8 +148,8 @@ Proof.
     apply (struct_validity ((TRec τ, TRec τ') :: A)). constructor; simpl; auto. apply (TRec_closed_unfold pτC). apply (TRec_closed_unfold pτ'C).
     (* apply (struct_validity ((TRec τ, TRec τ') :: A) τ.[TRec τ/] (TRec_closed_unfold pτC) τ'.[TRec τ'/] (TRec_closed_unfold pτ'C)). *)
     by apply cons_stand_unfold.
-    { apply t_step. apply left_lex. apply upper_bound_lt_rec_rec; auto. }
-Admitted.
+    { apply ord_left. apply upper_bound_lt_rec_rec; auto. }
+Qed.
 
 
 (** WF *)
@@ -112,7 +157,7 @@ Admitted.
 Next Obligation.
 Proof.
   apply measure_wf.
-  apply wf_clos_trans. apply wf_lexprod.
+  apply wf_lexprod.
   apply lt_wf. intros _.
-  apply wf_ord.
+  apply lt_wf.
 Qed.
